# baseURI: http://tutorial.topbraid.com/kgct
# imports: http://www.w3.org/2004/02/skos/core
# prefix: kgct

@prefix kgct: <http://tutorial.topbraid.com/kgct#> .
@prefix owl: <http://www.w3.org/2002/07/owl#> .
@prefix rdf: <http://www.w3.org/1999/02/22-rdf-syntax-ns#> .
@prefix rdfs: <http://www.w3.org/2000/01/rdf-schema#> .
@prefix skos: <http://www.w3.org/2004/02/skos/core#> .
@prefix xsd: <http://www.w3.org/2001/XMLSchema#> .

<http://tutorial.topbraid.com/kgct>
  rdf:type owl:Ontology ;
  owl:imports <http://www.w3.org/2004/02/skos/core> ;
  owl:versionInfo "Created with TopBraid Composer" ;
.
kgct:Statement_1
  rdf:type rdfs:Class ;
  rdfs:label "Statement 1" ;
  rdfs:subClassOf rdf:Statement ;
  skos:prefLabel "Statement 1" ;
.
kgct:bookDefinition
  rdf:type rdf:Property ;
  rdfs:comment "Points to a book chapter/section or online location where the subject term is defined" ;
  rdfs:domain skos:Concept ;
  rdfs:label "Book definition location" ;
.
kgct:bookReference
  rdf:type rdf:Property ;
  rdfs:comment "Points to a book chapter/section or online location where the subject term is referenced but not defined" ;
  rdfs:domain skos:Concept ;
  rdfs:label "Book reference location" ;
.
kgct:describes
  rdf:type rdf:Property ;
  rdfs:comment "Points to the public schema in which the term is formally defined" ;
  rdfs:domain skos:Concept ;
  rdfs:label "Term's rdf ontology source" ;
.
kgct:differentiates
  rdf:type rdf:Property ;
  rdfs:comment "Differentiates the term from a similar, complementary, or inverse term" ;
  rdfs:domain skos:Concept ;
  rdfs:label "Similar, complementary, or inverse term location" ;
.
kgct:example
  rdf:type rdf:Property ;
  rdfs:comment "Points to an example of the term used in code (e.g., Turtle, SPARQL)" ;
  rdfs:domain skos:Concept ;
  rdfs:label "Example of applied term" ;
.
