# baseURI: http://tutorial.topbraid.com/kgct
# imports: http://www.w3.org/2004/02/skos/core

@prefix bookclub: <https://dallemang.linked.data.world/d/bookclub/> .
@prefix kgct: <https://github.com/GlennClatworthy/kgct/blob/main/kgct.ttl#> .
@prefix owl: <http://www.w3.org/2002/07/owl#> .
@prefix rdf: <http://www.w3.org/1999/02/22-rdf-syntax-ns#> .
@prefix rdfs: <http://www.w3.org/2000/01/rdf-schema#> .
@prefix skos: <http://www.w3.org/2004/02/skos/core#> .
@prefix xsd: <http://www.w3.org/2001/XMLSchema#> .

<http://tutorial.topbraid.com/kgct>
  rdf:type owl:Ontology ;
  owl:imports <http://www.w3.org/2004/02/skos/core> ;
  owl:versionInfo "Created with TopBraid Composer" ;
.
<http://tutorial.topbraid.com/kgct#LearningPath>
  rdf:type rdfs:Class ;
  rdfs:comment "A series of concept references that point to one subdiscipline or subject (e.g., Turtle, SPARQL)" ;
  rdfs:subClassOf rdfs:Class ;
  skos:prefLabel "Learning path" ;
.
<http://tutorial.topbraid.com/kgct#PublicationSource>
  rdf:type rdfs:Class ;
  rdfs:label "Publication source" ;
  rdfs:subClassOf rdfs:Class ;
  skos:definition "A book, online source, or other resource making a statement about a skos:Concept" ;
.
<http://tutorial.topbraid.com/kgct#RDF>
  rdf:type skos:Concept ;
  <http://tutorial.topbraid.com/kgct#sourceDefinition> <http://tutorial.topbraid.com/kgct#_SiteW3CRDF> ;
  skos:altLabel "Resource Description Format" ;
  skos:prefLabel "RDF" ;
.
<http://tutorial.topbraid.com/kgct#Triple>
  rdf:type skos:Concept ;
  <http://tutorial.topbraid.com/kgct#ontologySource> "https://www.w3.org/1999/02/22-rdf-syntax-ns" ;
  <http://tutorial.topbraid.com/kgct#sourceDefinition> "https://dallemang.linked.data.world/d/bookclub/col-booktablecontent-chapter_section#row-booktablecontent-12" ;
  <http://tutorial.topbraid.com/kgct#sourceReference> "https://dallemang.linked.data.world/d/bookclub/col-booktablecontent-chapter_section#row-booktablecontent-12" ;
  skos:prefLabel "Triple" ;
.
<http://tutorial.topbraid.com/kgct#Triple001>
  rdf:type rdf:Statement ;
  <http://tutorial.topbraid.com/kgct#assertedBy> <http://tutorial.topbraid.com/kgct#_BookSWWO3rdEd> ;
  rdf:object "Tripleâ€”The fundamental data structure of RDF. A triple is made up of a subject, predicate, and object." ;
  rdf:predicate skos:definition ;
  rdf:subject <http://tutorial.topbraid.com/kgct#Triple> ;
  rdfs:label "Triple001" ;
.
<http://tutorial.topbraid.com/kgct#Triple002>
  rdf:type rdf:Statement ;
  <http://tutorial.topbraid.com/kgct#assertedBy> <http://tutorial.topbraid.com/kgct#_BookDOE1stEd> ;
  rdf:object "Triples assert relationships between things--e.g., JaneDoe worksFor Microsoft." ;
  rdf:predicate skos:definition ;
  rdf:subject <http://tutorial.topbraid.com/kgct#Triple> ;
  rdfs:label "Triple002" ;
.
<http://tutorial.topbraid.com/kgct#_BookDOE1stEd>
  rdf:type <http://tutorial.topbraid.com/kgct#PublicationSource> ;
  <http://tutorial.topbraid.com/kgct#sourceURI> "https://www.morganclaypool.com/doi/abs/10.2200/S00824ED1V01Y201801WBE017" ;
  rdfs:label "Demystifying OWL for the Enterprise" ;
.
<http://tutorial.topbraid.com/kgct#_BookSWWO3rdEd>
  rdf:type <http://tutorial.topbraid.com/kgct#PublicationSource> ;
  <http://tutorial.topbraid.com/kgct#sourceURI> "https://www.morganclaypoolpublishers.com/catalog_Orig/product_info.php?products_id=1564" ;
  rdfs:label "Semantic Web for the Working Ontologist, Third Edition" ;
.
<http://tutorial.topbraid.com/kgct#_PathRDFGeneral>
  rdf:type <http://tutorial.topbraid.com/kgct#LearningPath> ;
  rdfs:label " Path RDFGeneral" ;
.
<http://tutorial.topbraid.com/kgct#_PathRDFSPARQL>
  rdf:type <http://tutorial.topbraid.com/kgct#LearningPath> ;
  rdfs:label " Path RDFGeneral" ;
.
<http://tutorial.topbraid.com/kgct#_SiteW3CRDF>
  rdf:type <http://tutorial.topbraid.com/kgct#PublicationSource> ;
  <http://tutorial.topbraid.com/kgct#sourceURI> "https://www.w3.org/RDF/" ;
  rdfs:label "Resource Description Framework page on W3C" ;
.
<http://tutorial.topbraid.com/kgct#assertedBy>
  rdf:type rdf:Property ;
  rdfs:comment "Points to the source of an assertion about a concept for purposes of reification" ;
  rdfs:domain skos:Concept ;
  rdfs:label "AssertedBy" ;
.
<http://tutorial.topbraid.com/kgct#differentiates>
  rdf:type rdf:Property ;
  rdfs:comment "Differentiates the term from a similar, complementary, or inverse term" ;
  rdfs:domain skos:Concept ;
  rdfs:label "Similar, complementary, or inverse term location" ;
.
<http://tutorial.topbraid.com/kgct#example>
  rdf:type rdf:Property ;
  rdfs:comment "Points to an example of the term used in code (e.g., Turtle, SPARQL)" ;
  rdfs:domain skos:Concept ;
  rdfs:label "Example of applied term" ;
.
<http://tutorial.topbraid.com/kgct#inLearningPath>
  rdf:type rdf:Property ;
  rdfs:comment "Points to a subset of all resources focusing on one subject or area of instruction" ;
  rdfs:domain skos:Concept ;
  rdfs:label "In Learning Path" ;
.
<http://tutorial.topbraid.com/kgct#ontologySource>
  rdf:type rdf:Property ;
  rdfs:comment "Points to the public URI of the schema in which the term is formally defined" ;
  rdfs:domain skos:Concept ;
  rdfs:label "Concept URI" ;
.
<http://tutorial.topbraid.com/kgct#sourceDefinition>
  rdf:type rdf:Property ;
  rdfs:comment "Points to a book chapter/section or online location where the subject term is defined" ;
  rdfs:domain skos:Concept ;
  rdfs:label "Book definition location" ;
.
<http://tutorial.topbraid.com/kgct#sourceReference>
  rdf:type rdf:Property ;
  rdfs:comment "Points to a book chapter/section or online location where the subject term is referenced but not necessarily defined" ;
  rdfs:domain skos:Concept ;
  rdfs:label "Book reference location" ;
.
<http://tutorial.topbraid.com/kgct#sourceURI>
  rdf:type rdf:Property ;
  rdfs:comment "Points to the URI of the book's publisher's site or other reference source" ;
  rdfs:label "Source reference location" ;
.
